src/impl/TLS13.KeySchedule.fst
@@ -1,0 +1,383 @@
+module TLS13.KeySchedule
+
+#lang-pulse
+
+open Pulse.Lib.Pervasives
+open Pulse.Lib.Array.PtsTo
+
+module A = Pulse.Lib.Array.PtsTo
+module B = TLS13.Bytes
+module Crypto = TLS13.Crypto
+module K = TLS13.Keys
+module Seq = FStar.Seq
+module SZ = FStar.SizeT
+module U8 = FStar.UInt8
+
+inline_for_extraction
+let zero_u8 : U8.t = U8.uint_to_t 0
+
+noextract
+let label_derived_seq : B.bytes = K.label_derived
+noextract
+let label_c_hs_traffic_seq : B.bytes = K.label_c_hs_traffic
+noextract
+let label_s_hs_traffic_seq : B.bytes = K.label_s_hs_traffic
+noextract
+let label_c_ap_traffic_seq : B.bytes = K.label_c_ap_traffic
+noextract
+let label_s_ap_traffic_seq : B.bytes = K.label_s_ap_traffic
+noextract
+let label_finished_seq : B.bytes = K.label_finished
+noextract
+let label_key_seq : B.bytes = K.label_key
+noextract
+let label_iv_seq : B.bytes = K.label_iv
+
+inline_for_extraction
+fn write_label_derived (lbl: array U8.t)
+  requires pts_to lbl (Seq.create 7 zero_u8)
+  ensures pts_to lbl label_derived_seq
+{
+  lbl.(0sz) <- U8.uint_to_t 0x64;
+  lbl.(1sz) <- U8.uint_to_t 0x65;
+  lbl.(2sz) <- U8.uint_to_t 0x72;
+  lbl.(3sz) <- U8.uint_to_t 0x69;
+  lbl.(4sz) <- U8.uint_to_t 0x76;
+  lbl.(5sz) <- U8.uint_to_t 0x65;
+  lbl.(6sz) <- U8.uint_to_t 0x64;
+  with s. assert (pts_to lbl s);
+  assert_norm (s == label_derived_seq);
+  assert (pure (s == label_derived_seq));
+}
+
+inline_for_extraction
+fn write_label_c_hs_traffic (lbl: array U8.t)
+  requires pts_to lbl (Seq.create 12 zero_u8)
+  ensures pts_to lbl label_c_hs_traffic_seq
+{
+  lbl.(0sz) <- U8.uint_to_t 0x63;
+  lbl.(1sz) <- U8.uint_to_t 0x20;
+  lbl.(2sz) <- U8.uint_to_t 0x68;
+  lbl.(3sz) <- U8.uint_to_t 0x73;
+  lbl.(4sz) <- U8.uint_to_t 0x20;
+  lbl.(5sz) <- U8.uint_to_t 0x74;
+  lbl.(6sz) <- U8.uint_to_t 0x72;
+  lbl.(7sz) <- U8.uint_to_t 0x61;
+  lbl.(8sz) <- U8.uint_to_t 0x66;
+  lbl.(9sz) <- U8.uint_to_t 0x66;
+  lbl.(10sz) <- U8.uint_to_t 0x69;
+  lbl.(11sz) <- U8.uint_to_t 0x63;
+  with s. assert (pts_to lbl s);
+  assert_norm (s == label_c_hs_traffic_seq);
+  assert (pure (s == label_c_hs_traffic_seq));
+}
+
+inline_for_extraction
+fn write_label_s_hs_traffic (lbl: array U8.t)
+  requires pts_to lbl (Seq.create 12 zero_u8)
+  ensures pts_to lbl label_s_hs_traffic_seq
+{
+  lbl.(0sz) <- U8.uint_to_t 0x73;
+  lbl.(1sz) <- U8.uint_to_t 0x20;
+  lbl.(2sz) <- U8.uint_to_t 0x68;
+  lbl.(3sz) <- U8.uint_to_t 0x73;
+  lbl.(4sz) <- U8.uint_to_t 0x20;
+  lbl.(5sz) <- U8.uint_to_t 0x74;
+  lbl.(6sz) <- U8.uint_to_t 0x72;
+  lbl.(7sz) <- U8.uint_to_t 0x61;
+  lbl.(8sz) <- U8.uint_to_t 0x66;
+  lbl.(9sz) <- U8.uint_to_t 0x66;
+  lbl.(10sz) <- U8.uint_to_t 0x69;
+  lbl.(11sz) <- U8.uint_to_t 0x63;
+  with s. assert (pts_to lbl s);
+  assert_norm (s == label_s_hs_traffic_seq);
+  assert (pure (s == label_s_hs_traffic_seq));
+}
+
+inline_for_extraction
+fn write_label_c_ap_traffic (lbl: array U8.t)
+  requires pts_to lbl (Seq.create 12 zero_u8)
+  ensures pts_to lbl label_c_ap_traffic_seq
+{
+  lbl.(0sz) <- U8.uint_to_t 0x63;
+  lbl.(1sz) <- U8.uint_to_t 0x20;
+  lbl.(2sz) <- U8.uint_to_t 0x61;
+  lbl.(3sz) <- U8.uint_to_t 0x70;
+  lbl.(4sz) <- U8.uint_to_t 0x20;
+  lbl.(5sz) <- U8.uint_to_t 0x74;
+  lbl.(6sz) <- U8.uint_to_t 0x72;
+  lbl.(7sz) <- U8.uint_to_t 0x61;
+  lbl.(8sz) <- U8.uint_to_t 0x66;
+  lbl.(9sz) <- U8.uint_to_t 0x66;
+  lbl.(10sz) <- U8.uint_to_t 0x69;
+  lbl.(11sz) <- U8.uint_to_t 0x63;
+  with s. assert (pts_to lbl s);
+  assert_norm (s == label_c_ap_traffic_seq);
+  assert (pure (s == label_c_ap_traffic_seq));
+}
+
+inline_for_extraction
+fn write_label_s_ap_traffic (lbl: array U8.t)
+  requires pts_to lbl (Seq.create 12 zero_u8)
+  ensures pts_to lbl label_s_ap_traffic_seq
+{
+  lbl.(0sz) <- U8.uint_to_t 0x73;
+  lbl.(1sz) <- U8.uint_to_t 0x20;
+  lbl.(2sz) <- U8.uint_to_t 0x61;
+  lbl.(3sz) <- U8.uint_to_t 0x70;
+  lbl.(4sz) <- U8.uint_to_t 0x20;
+  lbl.(5sz) <- U8.uint_to_t 0x74;
+  lbl.(6sz) <- U8.uint_to_t 0x72;
+  lbl.(7sz) <- U8.uint_to_t 0x61;
+  lbl.(8sz) <- U8.uint_to_t 0x66;
+  lbl.(9sz) <- U8.uint_to_t 0x66;
+  lbl.(10sz) <- U8.uint_to_t 0x69;
+  lbl.(11sz) <- U8.uint_to_t 0x63;
+  with s. assert (pts_to lbl s);
+  assert_norm (s == label_s_ap_traffic_seq);
+  assert (pure (s == label_s_ap_traffic_seq));
+}
+
+inline_for_extraction
+fn write_label_finished (lbl: array U8.t)
+  requires pts_to lbl (Seq.create 8 zero_u8)
+  ensures pts_to lbl label_finished_seq
+{
+  lbl.(0sz) <- U8.uint_to_t 0x66;
+  lbl.(1sz) <- U8.uint_to_t 0x69;
+  lbl.(2sz) <- U8.uint_to_t 0x6e;
+  lbl.(3sz) <- U8.uint_to_t 0x69;
+  lbl.(4sz) <- U8.uint_to_t 0x73;
+  lbl.(5sz) <- U8.uint_to_t 0x68;
+  lbl.(6sz) <- U8.uint_to_t 0x65;
+  lbl.(7sz) <- U8.uint_to_t 0x64;
+  with s. assert (pts_to lbl s);
+  assert_norm (s == label_finished_seq);
+  assert (pure (s == label_finished_seq));
+}
+
+inline_for_extraction
+fn write_label_key (lbl: array U8.t)
+  requires pts_to lbl (Seq.create 3 zero_u8)
+  ensures pts_to lbl label_key_seq
+{
+  lbl.(0sz) <- U8.uint_to_t 0x6b;
+  lbl.(1sz) <- U8.uint_to_t 0x65;
+  lbl.(2sz) <- U8.uint_to_t 0x79;
+  with s. assert (pts_to lbl s);
+  assert_norm (s == label_key_seq);
+  assert (pure (s == label_key_seq));
+}
+
+inline_for_extraction
+fn write_label_iv (lbl: array U8.t)
+  requires pts_to lbl (Seq.create 2 zero_u8)
+  ensures pts_to lbl label_iv_seq
+{
+  lbl.(0sz) <- U8.uint_to_t 0x69;
+  lbl.(1sz) <- U8.uint_to_t 0x76;
+  with s. assert (pts_to lbl s);
+  assert_norm (s == label_iv_seq);
+  assert (pure (s == label_iv_seq));
+}
+
+fn derived_secret
+  (secret: array U8.t)
+  (out: array U8.t)
+  requires pts_to secret 'secret_bytes **
+           pts_to out 'old **
+           pure (B.length 'secret_bytes == 32 /\ B.length 'old == 32)
+  ensures pts_to secret 'secret_bytes **
+          pts_to out (K.derived_secret (Ghost.reveal 'secret_bytes))
+{
+  let empty_hash = A.alloc zero_u8 32sz;
+  Crypto.sha256_empty empty_hash;
+
+  let lbl = A.alloc zero_u8 7sz;
+  write_label_derived lbl;
+  Crypto.hkdf_expand_label secret lbl 7sz empty_hash 32sz out 32sz;
+
+  A.free lbl;
+  A.free empty_hash;
+}
+
+fn handshake_secret
+  (early: array U8.t)
+  (shared: array U8.t)
+  (shared_len: SZ.t)
+  (out: array U8.t)
+  requires pts_to early 'early_bytes **
+           pts_to shared 'shared_bytes **
+           pts_to out 'old **
+           pure (B.length 'early_bytes == 32 /\
+                 B.length 'shared_bytes == SZ.v shared_len /\
+                 B.length 'old == 32)
+  ensures pts_to early 'early_bytes **
+          pts_to shared 'shared_bytes **
+          pts_to out (K.handshake_secret (Ghost.reveal 'early_bytes) (Ghost.reveal 'shared_bytes))
+{
+  let derived = A.alloc zero_u8 32sz;
+  derived_secret early derived;
+  Crypto.hkdf_extract derived 32sz shared shared_len out;
+  A.free derived;
+}
+
+fn master_secret
+  (handshake: array U8.t)
+  (out: array U8.t)
+  requires pts_to handshake 'handshake_bytes **
+           pts_to out 'old **
+           pure (B.length 'handshake_bytes == 32 /\ B.length 'old == 32)
+  ensures pts_to handshake 'handshake_bytes **
+          pts_to out (K.master_secret (Ghost.reveal 'handshake_bytes))
+{
+  let derived = A.alloc zero_u8 32sz;
+  derived_secret handshake derived;
+  let zero = A.alloc zero_u8 32sz;
+  Crypto.hkdf_extract derived 32sz zero 32sz out;
+  A.free zero;
+  A.free derived;
+}
+
+fn client_handshake_traffic_secret
+  (handshake: array U8.t)
+  (transcript_hash: array U8.t)
+  (out: array U8.t)
+  requires pts_to handshake 'handshake_bytes **
+           pts_to transcript_hash 'hash_bytes **
+           pts_to out 'old **
+           pure (B.length 'handshake_bytes == 32 /\
+                 B.length 'hash_bytes == 32 /\
+                 B.length 'old == 32)
+  ensures pts_to handshake 'handshake_bytes **
+          pts_to transcript_hash 'hash_bytes **
+          pts_to out (K.client_handshake_traffic_secret
+                        (Ghost.reveal 'handshake_bytes)
+                        (Ghost.reveal 'hash_bytes))
+{
+  let lbl = A.alloc zero_u8 12sz;
+  write_label_c_hs_traffic lbl;
+  Crypto.hkdf_expand_label handshake lbl 12sz transcript_hash 32sz out 32sz;
+  A.free lbl;
+}
+
+fn server_handshake_traffic_secret
+  (handshake: array U8.t)
+  (transcript_hash: array U8.t)
+  (out: array U8.t)
+  requires pts_to handshake 'handshake_bytes **
+           pts_to transcript_hash 'hash_bytes **
+           pts_to out 'old **
+           pure (B.length 'handshake_bytes == 32 /\
+                 B.length 'hash_bytes == 32 /\
+                 B.length 'old == 32)
+  ensures pts_to handshake 'handshake_bytes **
+          pts_to transcript_hash 'hash_bytes **
+          pts_to out (K.server_handshake_traffic_secret
+                        (Ghost.reveal 'handshake_bytes)
+                        (Ghost.reveal 'hash_bytes))
+{
+  let lbl = A.alloc zero_u8 12sz;
+  write_label_s_hs_traffic lbl;
+  Crypto.hkdf_expand_label handshake lbl 12sz transcript_hash 32sz out 32sz;
+  A.free lbl;
+}
+
+fn client_application_traffic_secret
+  (master: array U8.t)
+  (transcript_hash: array U8.t)
+  (out: array U8.t)
+  requires pts_to master 'master_bytes **
+           pts_to transcript_hash 'hash_bytes **
+           pts_to out 'old **
+           pure (B.length 'master_bytes == 32 /\
+                 B.length 'hash_bytes == 32 /\
+                 B.length 'old == 32)
+  ensures pts_to master 'master_bytes **
+          pts_to transcript_hash 'hash_bytes **
+          pts_to out (K.client_application_traffic_secret
+                        (Ghost.reveal 'master_bytes)
+                        (Ghost.reveal 'hash_bytes))
+{
+  let lbl = A.alloc zero_u8 12sz;
+  write_label_c_ap_traffic lbl;
+  Crypto.hkdf_expand_label master lbl 12sz transcript_hash 32sz out 32sz;
+  A.free lbl;
+}
+
+fn server_application_traffic_secret
+  (master: array U8.t)
+  (transcript_hash: array U8.t)
+  (out: array U8.t)
+  requires pts_to master 'master_bytes **
+           pts_to transcript_hash 'hash_bytes **
+           pts_to out 'old **
+           pure (B.length 'master_bytes == 32 /\
+                 B.length 'hash_bytes == 32 /\
+                 B.length 'old == 32)
+  ensures pts_to master 'master_bytes **
+          pts_to transcript_hash 'hash_bytes **
+          pts_to out (K.server_application_traffic_secret
+                        (Ghost.reveal 'master_bytes)
+                        (Ghost.reveal 'hash_bytes))
+{
+  let lbl = A.alloc zero_u8 12sz;
+  write_label_s_ap_traffic lbl;
+  Crypto.hkdf_expand_label master lbl 12sz transcript_hash 32sz out 32sz;
+  A.free lbl;
+}
+
+fn finished_verify_data
+  (base_key: array U8.t)
+  (transcript_hash: array U8.t)
+  (out: array U8.t)
+  requires pts_to base_key 'base_key_bytes **
+          pts_to transcript_hash 'hash_bytes **
+          pts_to out 'old **
+          pure (B.length 'base_key_bytes == 32 /\
+                B.length 'hash_bytes == 32 /\
+                B.length 'old == 32)
+  ensures pts_to base_key 'base_key_bytes **
+          pts_to transcript_hash 'hash_bytes **
+          pts_to out (K.finished_verify_data
+                       (Ghost.reveal 'base_key_bytes)
+                       (Ghost.reveal 'hash_bytes))
+{
+  let lbl = A.alloc zero_u8 8sz;
+  write_label_finished lbl;
+  let finished_key = A.alloc zero_u8 32sz;
+  Crypto.hkdf_expand_label_empty_context base_key lbl 8sz finished_key 32sz;
+  Crypto.hmac_sha256 finished_key 32sz transcript_hash 32sz out;
+  A.free finished_key;
+  A.free lbl;
+}
+
+fn derive_traffic_key
+  (traffic_secret: array U8.t)
+  (out: array U8.t)
+  requires pts_to traffic_secret 'secret_bytes **
+          pts_to out 'old **
+           pure (B.length 'secret_bytes == 32 /\ B.length 'old == 32)
+  ensures pts_to traffic_secret 'secret_bytes **
+          pts_to out (K.derive_aead_key (Ghost.reveal 'secret_bytes))
+{
+  let lbl = A.alloc zero_u8 3sz;
+  write_label_key lbl;
+  Crypto.hkdf_expand_label_empty_context traffic_secret lbl 3sz out 32sz;
+  A.free lbl;
+}
+
+fn derive_traffic_iv
+  (traffic_secret: array U8.t)
+  (out: array U8.t)
+  requires pts_to traffic_secret 'secret_bytes **
+           pts_to out 'old **
+           pure (B.length 'secret_bytes == 32 /\ B.length 'old == 12)
+  ensures pts_to traffic_secret 'secret_bytes **
+          pts_to out (K.derive_aead_iv (Ghost.reveal 'secret_bytes))
+{
+  let lbl = A.alloc zero_u8 2sz;
+  write_label_iv lbl;
+  Crypto.hkdf_expand_label_empty_context traffic_secret lbl 2sz out 12sz;
+  A.free lbl;
+}
