Makefile
@@ -47,6 +47,7 @@ IMPL_FILES = \
   src/impl/TLS13.Connection.StateDriver.fst \
   src/impl/TLS13.Crypto.fsti \
   src/impl/TLS13.KeySchedule.fsti \
+  src/impl/TLS13.KeySchedule.fst \
   src/impl/TLS13.X509.fsti \
   src/impl/TLS13.Record.fsti \
   src/impl/TLS13.Parse.fsti \
